src/core/bir_typing_expScript.sml
@@ -3,7 +3,7 @@ open wordsTheory bitstringTheory;
 open bir_auxiliaryTheory bir_immTheory bir_valuesTheory;
 open bir_imm_expTheory bir_mem_expTheory bir_envTheory;
 open bir_expTheory
-open wordsLib;
+open wordsLib pred_setTheory;
 
 val _ = new_theory "bir_typing_exp";
 
@@ -337,5 +337,168 @@ GEN_TAC >> Induct >> (
   ASM_SIMP_TAC (std_ss++bir_val_ss) []
 ));
 
+
+(* --------------------------- *)
+(*  EXISTENCE OF SUITABLE ENVS *)
+(* --------------------------- *)
+
+
+val bir_default_value_of_type_def = Define `
+  (bir_default_value_of_type (BType_Imm s) = BVal_Imm (n2bs 0 s)) /\
+  (bir_default_value_of_type (BType_Mem a_s v_s) = BVal_Mem a_s v_s (K 0))`;
+
+val bir_default_value_of_type_SPEC = store_thm ("bir_default_value_of_type_SPEC",
+  ``!ty. type_of_bir_val (bir_default_value_of_type ty) = SOME ty``,
+
+Cases >> (
+  SIMP_TAC std_ss [bir_default_value_of_type_def, type_of_bir_val_def, type_of_n2bs]
+));
+
+
+val bir_immtype_t_LIST_def = Define `bir_immtype_t_LIST = ^(listSyntax.mk_list (bir_immSyntax.bir_immtype_t_list, bir_immSyntax.bir_immtype_t_ty))`;
+
+
+val bir_immtype_t_LIST_THM = store_thm ("bir_immtype_t_LIST_THM",
+  ``!s. MEM s bir_immtype_t_LIST``,
+Cases >> SIMP_TAC list_ss [bir_immtype_t_LIST_def]);
+
+val bir_immtype_t_UNIV_SPEC = store_thm ("bir_immtype_t_UNIV_SPEC",
+  ``(UNIV:bir_immtype_t set) = set bir_immtype_t_LIST``,
+
+SIMP_TAC list_ss [EXTENSION, bir_immtype_t_LIST_THM, IN_UNIV]);
+
+
+val bir_immtype_t_FINITE_UNIV = store_thm ("bir_immtype_t_FINITE_UNIV",
+  ``FINITE (UNIV : (bir_immtype_t set))``,
+REWRITE_TAC[bir_immtype_t_UNIV_SPEC, listTheory.FINITE_LIST_TO_SET]);
+
+
+
+val bir_type_t_LIST_def = (let
+  open bir_valuesSyntax bir_immSyntax
+  val imm_types = List.map mk_BType_Imm bir_immtype_t_list
+  val mem_types = List.map mk_BType_Mem (flatten (
+     List.map (fn v1 => List.map (fn v2 => (v1, v2)) bir_immtype_t_list) bir_immtype_t_list))
+  val t = listSyntax.mk_list (imm_types @ mem_types, bir_type_t_ty)
+in
+  Define `bir_type_t_LIST = ^t`
+end);
+
+
+val bir_type_t_LIST_THM = store_thm ("bir_type_t_LIST_THM",
+  ``!ty. MEM ty bir_type_t_LIST``,
+
+SIMP_TAC list_ss [bir_type_t_LIST_def] >>
+SIMP_TAC (list_ss++DatatypeSimps.expand_type_quants_ss[``:bir_immtype_t``, ``:bir_type_t``]) []);
+
+
+val bir_type_t_UNIV_SPEC = store_thm ("bir_type_t_UNIV_SPEC",
+  ``(UNIV:bir_type_t set) = set bir_type_t_LIST``,
+
+SIMP_TAC list_ss [EXTENSION, bir_type_t_LIST_THM, IN_UNIV]);
+
+
+val bir_type_t_FINITE_UNIV = store_thm ("bir_type_t_FINITE_UNIV",
+  ``FINITE (UNIV : (bir_type_t set))``,
+REWRITE_TAC[bir_type_t_UNIV_SPEC, listTheory.FINITE_LIST_TO_SET]);
+
+
+val bir_env_vars_are_initialised_FINITE = store_thm ("bir_env_vars_are_initialised_FINITE",
+  ``!vs env. bir_env_vars_are_initialised env vs ==> FINITE vs``,
+
+REPEAT STRIP_TAC >>
+Cases_on `env` >> rename1 `BEnv env` >>
+`IMAGE bir_var_name vs SUBSET FDOM env` by (
+  FULL_SIMP_TAC std_ss [bir_env_vars_are_initialised_def, SUBSET_DEF, IN_IMAGE,
+    PULL_EXISTS] >>
+  REPEAT STRIP_TAC >>
+  rename1 `v IN vs` >>
+  Q.PAT_X_ASSUM `!v. _` (MP_TAC o Q.SPEC `v`) >>
+  Cases_on `v` >> rename1 `BVar vn vty` >>
+  ASM_SIMP_TAC std_ss [bir_env_var_is_initialised_def, bir_env_lookup_def,
+    finite_mapTheory.flookup_thm, PULL_EXISTS, bir_var_name_def]
+) >>
+
+`FINITE (IMAGE bir_var_name vs)` by METIS_TAC[
+  SUBSET_FINITE, finite_mapTheory.FDOM_FINITE] >>
+
+Q.ABBREV_TAC `VS = BIGUNION (IMAGE (\vn. IMAGE (\ty. BVar vn ty) UNIV) (IMAGE bir_var_name vs))` >>
+`vs SUBSET VS` by (
+  Q.UNABBREV_TAC `VS` >>
+  SIMP_TAC std_ss [SUBSET_DEF, IN_BIGUNION, IN_IMAGE, PULL_EXISTS, IN_UNIV] >>
+  REPEAT STRIP_TAC >>
+  rename1 `v IN vs` >>
+  Q.EXISTS_TAC `v` >>
+  Q.EXISTS_TAC `bir_var_type v` >>
+  Cases_on `v` >>
+  ASM_SIMP_TAC std_ss [bir_var_type_def, bir_var_name_def]
+) >>
+
+`FINITE VS` suffices_by METIS_TAC[SUBSET_FINITE] >>
+Q.UNABBREV_TAC `VS` >>
+SIMP_TAC std_ss [FINITE_BIGUNION_EQ, IN_IMAGE, PULL_EXISTS] >>
+METIS_TAC[IMAGE_FINITE, bir_type_t_FINITE_UNIV]);
+
+
+
+val bir_var_set_is_well_typed_def = Define `bir_var_set_is_well_typed vs <=>
+  (!v1 v2. (v1 IN vs /\ v2 IN vs /\ (bir_var_name v1 = bir_var_name v2)) ==>
+           (bir_var_type v1 = bir_var_type v2))`;
+
+val bir_var_set_is_well_typed_INJ_DEF = store_thm ("bir_var_set_is_well_typed_INJ_DEF",
+  ``bir_var_set_is_well_typed vs <=> INJ bir_var_name vs UNIV``,
+
+SIMP_TAC std_ss [bir_var_set_is_well_typed_def, INJ_DEF, IN_UNIV,
+  bir_var_eq_EXPAND] >>
+METIS_TAC[]);
+
+
+val bir_env_vars_are_initialised_WELL_TYPED = store_thm ("bir_env_vars_are_initialised_WELL_TYPED",
+  ``!vs env. bir_env_vars_are_initialised env vs ==> bir_var_set_is_well_typed vs``,
+
+  SIMP_TAC std_ss [bir_var_set_is_well_typed_def, bir_env_vars_are_initialised_def] >>
+  REPEAT STRIP_TAC >>
+  Cases_on `v1` >> Cases_on `v2` >>
+  rename1 `bir_var_name (BVar vn1 vty1) = bir_var_name (BVar vn2 vty2)` >>
+  FULL_SIMP_TAC std_ss [bir_var_name_def, bir_var_type_def] >>
+
+
+  `bir_env_var_is_initialised env (BVar vn2 vty1)` by METIS_TAC[] >>
+  `bir_env_var_is_initialised env (BVar vn2 vty2)` by METIS_TAC[] >>
+  FULL_SIMP_TAC std_ss [bir_env_var_is_initialised_def] >>
+  FULL_SIMP_TAC std_ss []
+);
+
+
+val bir_env_vars_are_initialised_ENV_EXISTS = store_thm ("bir_env_vars_are_initialised_ENV_EXISTS",
+  ``!vs. (?env. bir_env_vars_are_initialised env vs) <=> (FINITE vs /\ bir_var_set_is_well_typed vs)``,
+
+GEN_TAC >> EQ_TAC >- (
+  METIS_TAC[bir_env_vars_are_initialised_WELL_TYPED, bir_env_vars_are_initialised_FINITE]
+) >>
+REPEAT STRIP_TAC >>
+Q.ABBREV_TAC `VF = (\v. (bir_var_type v, SOME (bir_default_value_of_type (bir_var_type v))))` >>
+Q.ABBREV_TAC `M1 = FUN_FMAP VF vs` >>
+EXISTS_TAC ``BEnv (MAP_KEYS bir_var_name M1)`` >>
+
+`FDOM M1 = vs` by METIS_TAC[finite_mapTheory.FDOM_FMAP] >>
+`INJ bir_var_name (FDOM M1) UNIV` by METIS_TAC [bir_var_set_is_well_typed_INJ_DEF] >>
+
+SIMP_TAC std_ss [bir_env_vars_are_initialised_def]  >>
+Cases >> rename1 `BVar vn vty` >>
+ASM_SIMP_TAC std_ss [bir_env_var_is_initialised_def,
+  bir_env_lookup_def, finite_mapTheory.FLOOKUP_MAP_KEYS] >>
+REPEAT STRIP_TAC >>
+
+`!v'. ((vn = bir_var_name v') ∧ v' IN vs) <=> (v' = BVar vn vty)` by (
+  FULL_SIMP_TAC std_ss [INJ_DEF, IN_UNIV] >>
+  METIS_TAC[bir_var_name_def]
+) >>
+ASM_SIMP_TAC std_ss [] >>
+
+Q.UNABBREV_TAC `M1` >>
+Q.UNABBREV_TAC `VF` >>
+ASM_SIMP_TAC std_ss [finite_mapTheory.FLOOKUP_FUN_FMAP,
+  bir_default_value_of_type_SPEC, bir_var_type_def]);
 
 val _ = export_theory();
